\chapter{karxmAgata saMKeyxgaLa GanagaLa motatx kaMDuhiDiyuvudu}
\vskip -20pt

$$
1^3+2^3+3^3\ldots n^3
$$
\begin{align*}
&n^4 - (n-1)^4 = 4n^3 - 6n^2 +4n -1\\
&4n^{3}-6n^2 + 4n -1 = n^4 - (n-1)^4\\
&4S_{3} - 6S_{2} +4S_{1} -n = n^4\\
&4S_{3}-6S_{2} +4S_{1}-n = n^4 \qquad\text{($1=n$, $n-n =0$)}\\
&4S_{3} = n^4 +6S_{2} -4S_{1} +n
\end{align*}
\begin{align*}
&=n^4+6\cdot \frac{n(n+1)(2n+1)}{6} -4 \frac{n(n+1)}{2}+n\\
&=n\left[n^3 + \left(2n^2 + n+2n +1\right) - 2(n+1) +1\right]\\
&=n\left[n^3+2n^2+n+2n+1-2n-2+1\right]\\
&=n\left[n^3+2n^{2}+n\right]\\
&=n^2\left[n^2+2n+1\right]\\
S_3&= \frac{n^2(n+1)^2}{4}\\
&=\left[\frac{n}{2}(n+1)\right]^2\\
&=\frac{n^2}{4}(n+1)^2
\end{align*}
