\chapter{karxmAgata saMKeyxgaLa vagaRgaLa motatxvanunx kaMDuhiDiyuvudu}

$$
1^2+2^2+3^2\ldots n^2
$$
\begin{gather*}
n^3 -(n-1)^3 = n^3 - n^2+3n^2 - 3n+1\\
3n^2-3n+1 = n^3-(n-1)^3\\
3S_{2}-3S_{1} +n = n^3 \qquad\text{($1=n$)}\\
3S_{2} = n^3+ 3S_{1}-n
\end{gather*}
\begin{align*}
&n^3 + 3 \cdot \frac{n(n+1)}{2} -n\\
&=n\left[n^2+\frac {3(n+1)}{2}-1\right]\\
&=n \left[n^2+\frac{3n+3}{2}-1\right]\\
&=n\left[\frac{2n^2 + 3n + 3 - 2}{2}\right]\\
&=n\left[\frac{(n+1)(2n+1)}{2}\right]\\
S_2 &=\frac{n(n+1)(2n+1)}{6}
\end{align*}
